setting up idg experiment (induction dependency graph) for running on aws

tools/idg/idg-gen-files.py
@@ -1,0 +1,47 @@
+#!/usr/bin/python3
+"""
+This file is meant to be run from BlockCacheSystem/ and it will generate many files for the IDG experiments
+
+Example run:
+python3 ../tools/idg/idg-gen-files.py
+
+"""
+
+lines = open('BlockSystem.i.dfy').read().splitlines()
+
+i_pre = 511
+i_post = 547
+
+assert '    && Inv1(s)' == lines[i_pre]
+assert '    && Inv1(s)' == lines[i_post]
+
+if False:
+    for i in range(32):
+        lines_i = lines[:]
+        lines_i[i_pre + i] = '// ' + lines_i[i_pre + i]
+        lines_i[i_post + i] = '// ' + lines_i[i_post + i]
+        fn = f'BlockSystem.{i}.i.dfy'
+        open(fn, 'w').write('\n'.join(lines_i))
+
+if False:
+    for j in range(32):
+        lines_ = lines[:]
+        lines_[i_pre + j] = '// ' + lines_[i_pre + j]
+        for k in range(32):
+            lines_[i_post + k] = '// ' + lines_[i_post + k]
+        fn = f'BlockSystem.none.{j}.i.dfy'
+        open(fn, 'w').write('\n'.join(lines_))
+
+if True:
+    needed = set([0, 1, 2, 3, 6, 7, 9, 10, 11, 14, 15, 16, 17, 19, 20, 28, 29, 30, 31])
+    for i in range(32):
+        for j in range(32):
+            if i == j or j in needed:
+                continue
+            lines_ = lines[:]
+            lines_[i_pre + j] = '// ' + lines_[i_pre + j]
+            for k in range(32):
+                if k != i:
+                    lines_[i_post + k] = '// ' + lines_[i_post + k]
+            fn = f'BlockSystem.{i}.{j}.i.dfy'
+            open(fn, 'w').write('\n'.join(lines_))
