tools/local-dafny.sh
@@ -1,4 +1,4 @@
 #! /bin/bash
 
 DIR="$( cd "$( dirname "${BASH_SOURCE[0]}" )" >/dev/null 2>&1 && pwd )"
-$DIR/../.dafny/bin/dafny "$@"
+time $DIR/../.dafny/bin/dafny "$@"
